Coq/src/ProgES.v
@@ -1,7 +1,7 @@
 Require Import Omega Setoid Program.Basics.
 From hahn Require Import Hahn.
 From promising Require Import Basic.
-From imm Require Import Events Prog ProgToExecution.
+From imm Require Import Events Prog Execution ProgToExecution.
 Require Import AuxDef.
 Require Import AuxRel.
 Require Import EventStructure.
@@ -32,7 +32,16 @@ Definition prog_init_K (prog : Prog.t) :=
        (prog_init_threads prog)).
 
 Definition prog_es_init (prog : Prog.t) :=
-  let loc_labs :=
-      map (fun l => Astore Xpln Opln l 0) (prog_locs prog)
+  ES.init (prog_locs prog) (prog_init_K prog).
+
+Definition prog_g_es_init (prog : Prog.t) (G : execution) :=
+  let glocs :=
+      flatten
+        (map (fun e =>
+                match e with
+                | InitEvent l => [l]
+                | _ => []
+                end)
+             (acts G))
   in
-  ES.init loc_labs (prog_init_K prog).
+  ES.init glocs (prog_init_K prog).
